# Matrix Multiplication Optimization

## Representations

Given three $n \times n$ matrices $\boldsymbol{A}$, $\boldsymbol{B}$, and $\boldsymbol{C}$.

$$
\begin{align}
\boldsymbol{C} & = \boldsymbol{A}\boldsymbol{B}
\\

\begin{bmatrix}
  c_{11} & c_{12} & \cdots & c_{1n} \\
  c_{21} & c_{22} & \cdots & c_{2n} \\
  \vdots  & \vdots  & \ddots & \vdots  \\
  c_{n1} & c_{n2} & \cdots & c_{nn} 
\end{bmatrix} & = 
\begin{bmatrix}
  a_{11} & a_{12} & \cdots & a_{1n} \\
  a_{21} & a_{22} & \cdots & a_{2n} \\
  \vdots  & \vdots  & \ddots & \vdots  \\
  a_{n1} & a_{n2} & \cdots & a_{nn} 
\end{bmatrix}
\begin{bmatrix}
  b_{11} & b_{12} & \cdots & b_{1n} \\
  b_{21} & b_{22} & \cdots & b_{2n} \\
  \vdots  & \vdots  & \ddots & \vdots  \\
  b_{n1} & b_{n2} & \cdots & b_{nn} 
\end{bmatrix}
\end{align}
$$

The multiplication can be achieved in a divide and conquer manner which operates on the submatrices.

$$
\begin{bmatrix}
  \boldsymbol{c}_{11} & \boldsymbol{c}_{12} & \cdots & \boldsymbol{c}_{1m} \\
  \boldsymbol{c}_{21} & \boldsymbol{c}_{22} & \cdots & \boldsymbol{c}_{2m} \\
  \vdots  & \vdots  & \ddots & \vdots  \\
  \boldsymbol{c}_{m1} & \boldsymbol{c}_{m2} & \cdots & \boldsymbol{c}_{mm} 
\end{bmatrix} = 
\begin{bmatrix}
  \boldsymbol{a}_{11} & \boldsymbol{a}_{12} & \cdots & \boldsymbol{a}_{1m} \\
  \boldsymbol{a}_{21} & \boldsymbol{a}_{22} & \cdots & \boldsymbol{a}_{2m} \\
  \vdots  & \vdots  & \ddots & \vdots  \\
  \boldsymbol{a}_{m1} & \boldsymbol{a}_{m2} & \cdots & \boldsymbol{a}_{mm} 
\end{bmatrix}
\begin{bmatrix}
  \boldsymbol{b}_{11} & \boldsymbol{b}_{12} & \cdots & \boldsymbol{b}_{1m} \\
  \boldsymbol{b}_{21} & \boldsymbol{b}_{22} & \cdots & \boldsymbol{b}_{2m} \\
  \vdots  & \vdots  & \ddots & \vdots  \\
  \boldsymbol{b}_{m1} & \boldsymbol{b}_{m2} & \cdots & \boldsymbol{b}_{mm} 
\end{bmatrix}
$$

The original calculation process of each submatrix $\boldsymbol{c}_{ij}$ is as follows.

$$
\boldsymbol{c}_{ij} = \sum^{m}_{k=1} \boldsymbol{a}_{ik} \cdot \boldsymbol{b}_{kj}, \quad \forall i, j \in [1, m]
\label{c_origin_calc}
$$

Considering the trace of the product of three matrices $\boldsymbol{A} \boldsymbol{B} \boldsymbol{C}$ where $\boldsymbol{A}$ is $\alpha \times \beta$, $\boldsymbol{B}$ is $\beta \times \gamma$, and $\boldsymbol{C}$ is $\gamma \times \alpha$.

$$
\begin{align}
\text{Tr}(\boldsymbol{A} \boldsymbol{B} \boldsymbol{C}) & = \text{Tr}\left(
\begin{bmatrix}
  a_{11} & a_{12} & \cdots & a_{1 \beta} \\
  a_{21} & a_{22} & \cdots & a_{2 \beta} \\
  \vdots  & \vdots  & \ddots & \vdots  \\
  a_{\alpha 1} & a_{\alpha 2} & \cdots & a_{\alpha \beta} 
\end{bmatrix}
\begin{bmatrix}
  b_{11} & b_{12} & \cdots & b_{1 \gamma} \\
  b_{21} & b_{22} & \cdots & b_{2 \gamma} \\
  \vdots  & \vdots  & \ddots & \vdots  \\
  b_{\beta 1} & b_{\beta 2} & \cdots & b_{\beta \gamma} 
\end{bmatrix}
\begin{bmatrix}
  c_{11} & c_{12} & \cdots & c_{1 \alpha} \\
  c_{21} & c_{22} & \cdots & c_{2 \alpha} \\
  \vdots  & \vdots  & \ddots & \vdots  \\
  c_{\gamma 1} & c_{\gamma 2} & \cdots & c_{\gamma \alpha} 
\end{bmatrix}
\right)
\\
& = \text{Tr}\left(
\begin{bmatrix}
  \sum\limits^{\beta}_{j=1} a_{1j} b_{j1} & \sum\limits^{\beta}_{j=1} a_{1j} b_{j2} & \cdots & \sum\limits^{\beta}_{j=1} a_{1j} b_{j \gamma} \\
  \sum\limits^{\beta}_{j=1} a_{2j} b_{j1} & \sum\limits^{\beta}_{j=1} a_{2j} b_{j2} & \cdots & \sum\limits^{\beta}_{j=1} a_{2j} b_{j \gamma} \\
  \vdots  & \vdots  & \ddots & \vdots  \\
  \sum\limits^{\beta}_{j=1} a_{\alpha j} b_{j1} & \sum\limits^{\beta}_{j=1} a_{\alpha j} b_{j2} & \cdots & \sum\limits^{\beta}_{j=1} a_{\alpha j} b_{j \gamma} 
\end{bmatrix}
\begin{bmatrix}
  c_{11} & c_{12} & \cdots & c_{1 \alpha} \\
  c_{21} & c_{22} & \cdots & c_{2 \alpha} \\
  \vdots  & \vdots  & \ddots & \vdots  \\
  c_{\gamma 1} & c_{\gamma 2} & \cdots & c_{\gamma \alpha} 
\end{bmatrix}
\right)
\\
& = \text{Tr}\left(
\begin{bmatrix}
  \sum\limits^{\beta}_{j=1} \sum\limits^{\gamma}_{k=1} a_{1j} b_{jk} c_{k1} & \cdots & \cdots & \cdots \\
  \vdots & \sum\limits^{\beta}_{j=1} \sum\limits^{\gamma}_{k=1} a_{2j} b_{jk} c_{k2} & \cdots & \cdots \\
  \vdots  & \vdots  & \ddots & \vdots  \\
  \vdots & \vdots & \cdots & \sum\limits^{\beta}_{j=1} \sum\limits^{\gamma}_{k=1} a_{\alpha j} b_{jk} c_{k \alpha} 
\end{bmatrix}
\right)
\\
& = \sum^{\alpha}_{i=1} \sum^{\beta}_{j=1} \sum^{\gamma}_{k=1} a_{ij} b_{jk} c_{ki}
\end{align}
$$


## Constructing Intermediates

We construct $u$ intermediates $\boldsymbol{M}_{v}, \forall 1 \le v \le u$, each of which is in the product-of-sum form and contains only single multiplication.
Let $p^{v}_{ij}, q^{v}_{ij} \in R, \forall v \in [1, u], \forall i, j \in [1, m]$ be proper constant scalar parameters to determine.
As long as $u < m^{3}$ is true, there will be less multiplications.

$$
\boldsymbol{M}_{v} = \left( \sum^{m}_{i=1} \sum^{m}_{j=1} p^{v}_{ij} \boldsymbol{a}_{ij} \right) \cdot \left( \sum^{m}_{i=1} \sum^{m}_{j=1} q^{v}_{ij} \boldsymbol{b}_{ij} \right), \quad \forall v \in [1, u]
$$


## Reformulating Expressions

We calculate each submatrix $\boldsymbol{c}_{ij}$ by adding the intermediates only.
Let $r^{v}_{ij} \in R, \forall v \in [1, u], \forall i, j \in [1, m]$ be proper constant scalar parameters to determine.

$$
\boldsymbol{c}_{ij} = \sum^{u}_{v=1} r^{v}_{ij} \boldsymbol{M}_{v}, \quad \forall i, j \in [1, m]
\label{c_new_calc}
$$


## Determining Parameters

In order to determine the proper constant scalar parameters $p^{v}_{ij}, q^{v}_{ij}, r^{v}_{ij} \in R, \forall v \in [1, u], \forall i, j \in [1, m]$, we combine Equations $(\ref{c_origin_calc})$ and $(\ref{c_new_calc})$.

$$
\sum^{m}_{k=1} \boldsymbol{a}_{ik} \cdot \boldsymbol{b}_{kj} = \sum^{u}_{v=1} r^{v}_{ij} \boldsymbol{M}_{v}, \quad \forall i, j \in [1, m]
$$

For each term $\boldsymbol{a}_{ik} \cdot \boldsymbol{b}_{kj}$ on the left-hand side, there are corresponding ones $r^{v}_{ij} p^{v}_{ik} q^{v}_{kj} \boldsymbol{a}_{ik} \cdot \boldsymbol{b}_{kj}, \forall v \in [1, u]$ on the right-hand side. Apparently, their coefficients must be equal.

$$
\sum^{u}_{v=1} r^{v}_{ij} p^{v}_{ik} q^{v}_{kj} = 1, \quad \forall i, j, k \in [1, m]
\label{coef_exist}
$$

Furthermore, for each term which does not appear on the left-hand side, there are still corresponding ones on the right-hand side, whose coefficients must be zero.

$$
\sum^{u}_{v=1} r^{v}_{ij} p^{v}_{i'k} q^{v}_{k'j'} = 0, \quad \forall i, i', j, j', k, k' \in [1, m], (i \ne i') \vee (j \ne j') \vee (k \ne k')
\label{coef_non_exist}
$$

In the literature, Equations $(\ref{coef_exist})$ and $(\ref{coef_non_exist})$ are usually combined into single formulation (Brent equations) by introducing $\delta_{ij} \leftarrow bool(i = j)$.

$$
\sum^{u}_{v=1} r^{v}_{ij} p^{v}_{i'k} q^{v}_{k'j'} = \delta_{ii'} \delta_{jj'} \delta_{kk'}, \quad \forall i, i', j, j', k, k' \in [1, m]
\label{coef_combine}
$$

Interestingly, most attempts for solving Equations $(\ref{coef_combine})$ when $m = 2, 3$ obtain ternary solutions in the literature, i.e., $p^{v}_{ij}, q^{v}_{ij}, r^{v}_{ij} \in \{-1, 0, 1\}, \forall v \in [1, u], \forall i, j \in [1, m]$.


## SAT Encoding

### Relaxed Model

It leads to a straightforward encoding if we only consider the state of "is involved or not" for each coefficient.
...

### Complete Model

In order to encode Equations $(\ref{coef_exist})$ and $(\ref{coef_non_exist})$ into Boolean expressions, we need to use a pair of binary variables to simulate the ternary values.

$$
\begin{array}{lll}
r^{v+}_{ij} = \text{bool}(r^{v}_{ij} = 1)  \quad & p^{v+}_{ij} = \text{bool}(p^{v}_{ij} = 1)  \quad & q^{v+}_{ij} = \text{bool}(q^{v}_{ij} = 1)\\
r^{v-}_{ij} = \text{bool}(r^{v}_{ij} = -1) \quad & p^{v-}_{ij} = \text{bool}(p^{v}_{ij} = -1) \quad & q^{v-}_{ij} = \text{bool}(q^{v}_{ij} = -1)
\end{array}
, \quad \forall v \in [1, u], \forall i, j \in [1, m]
$$

Naturally, the values of these pairs of binary variables are exclusive with each other.

$$
\bigwedge_{\substack{v \in [1, u] \\ i, j \in [1, m]}} \left( (\neg r^{v+}_{ij} \vee \neg r^{v-}_{ij}) \wedge  (\neg p^{v+}_{ij} \vee \neg p^{v-}_{ij}) \wedge (\neg q^{v+}_{ij} \vee \neg q^{v-}_{ij}) \right)
\label{exclusive}
$$

For each cubic product term, it is non-zero iff all of the three variables are non-zero.

$$
\text{NonZero}(v, i, i', j, j', k, k') = (r^{v+}_{ij} \vee r^{v-}_{ij}) \wedge (p^{v+}_{i'k} \vee p^{v-}_{i'k}) \wedge (q^{v+}_{k'j'} \vee q^{v-}_{k'j'})
$$

For a non-zero term, its sign depends on if the number of $-1$ is even or odd.

$$
\text{OddNegOne}(v, i, i', j, j', k, k') = r^{v-}_{ij} \oplus p^{v-}_{i'k} \oplus q^{v-}_{k'j'}
$$

$$
\text{EvenNegOne}(v, i, i', j, j', k, k') = r^{v-}_{ij} \oplus p^{v-}_{i'k} \oplus q^{v-}_{k'j'} \oplus 1
$$

Then, the numbers of positive ones $\text{Ones}(i, i', j, j', k, k')$ and negative ones $\text{NegOnes}(i, i', j, j', k, k')$ in each equation among Equations $(\ref{coef_exist})$ and $(\ref{coef_non_exist})$ can be counted as follows.

$$
\text{NegOnes}(i, i', j, j', k, k') = \sum^{u}_{v=1} \big( \text{NonZero}(v, i, i', j, j', k, k') \wedge \text{OddNegOne}(v, i, i', j, j', k, k') \big)
$$

$$
\text{Ones}(i, i', j, j', k, k') = \sum^{u}_{v=1} \big( \text{NonZero}(v, i, i', j, j', k, k') \wedge \text{EvenNegOne}(v, i, i', j, j', k, k') \big)
$$

In order to make both sides equal in Equations $(\ref{coef_exist})$ and $(\ref{coef_non_exist})$, the number of the ones and the negative ones must satisfy the following criteria.

$$
\text{Ones}(i, i, j, j, k, k) - \text{NegOnes}(i, i, j, j, k, k) = 1, \quad \forall i, j, k \in [1, m]
\label{coef_exist_cnf}
$$

$$
\text{Ones}(i, i', j, j', k, k') = \text{NegOnes}(i, i', j, j', k, k'), \quad \forall i, i', j, j', k, k' \in [1, m], (i \ne i') \vee (j \ne j') \vee (k \ne k')
\label{coef_non_exist_cnf}
$$

Then, Equations $(\ref{coef_exist})$ and $(\ref{coef_non_exist})$ are encoded into Equations $(\ref{exclusive})$,  $(\ref{coef_exist_cnf})$, and $(\ref{coef_non_exist_cnf})$.


## Mixed-Integer Programming

### Formulating Exclusive Or Operator

It is easy to convert Equations $(\ref{exclusive})$,  $(\ref{coef_exist_cnf})$, and $(\ref{coef_non_exist_cnf})$ into an MIP model. The only obstacle is the XOR operator.
Let $o^{v}_{ii'jj'kk'} \in \{0, 1\}, \forall v \in [1, u], \forall i, i', j, j', k, k' \in [1, m]$ indicate whether $(r^{v-}_{ij} + p^{v-}_{i'k} + q^{v-}_{k'j'}) \in \{1, 3\}$, i.e., $o^{v}_{ii'jj'kk'} = \text{OddNegOne}(v, i, i', j, j', k, k')$. Then $1 - o^{v}_{ii'jj'kk'}$ indicate whether $(r^{v-}_{ij} + p^{v-}_{i'k} + q^{v-}_{k'j'}) \in \{0, 2\}$, i.e., $1 - o^{v}_{ii'jj'kk'} = \text{EvenNegOne}(v, i, i', j, j', k, k')$, since a number must be either even or odd.
Let $y^{v}_{ii'jj'kk'} \in \{0, 1\}, \forall v \in [1, u], \forall i, i', j, j', k, k' \in [1, m]$ be the auxiliary variables for linearizing the or logic.

$$
r^{v-}_{ij} + p^{v-}_{i'k} + q^{v-}_{k'j'} = 2 y^{v}_{ii'jj'kk'} + o^{v}_{ii'jj'kk'}, \quad \forall v \in [1, u], \forall i, i', j, j', k, k' \in [1, m]
$$

### Other Logical Operators

For the rest parts, $\text{NonZero}(v, i, i', j, j', k, k')$ can be easily replaced with variables $z^{v}_{ii'jj'kk'} \in \{0, 1\}, \forall v \in [1, u], \forall i, i', j, j', k, k' \in [1, m]$ by applying the technique that $\left( y = \bigwedge^{n}_{i=1} x_{i} \right) \Leftrightarrow \left( 0 \le \sum^{n}_{i=1} x_{i} - n y \le n - 1 \right)$ (note that $x, y, n, i$ in this sentence are irrelevant to other contents in this document).

$$
3 z^{v}_{ii'jj'kk'} \le r^{v+}_{ij} + r^{v-}_{ij} + p^{v+}_{i'k} + p^{v-}_{i'k} + q^{v+}_{k'j'} + q^{v-}_{k'j'} \le 2 + z^{v}_{ii'jj'kk'}, \quad \forall v \in [1, u], \forall i, i', j, j', k, k' \in [1, m]
\label{non_zero_var}
$$

Equations $(\ref{non_zero_var})$ are sufficient to derive $z^{v}_{ii'jj'kk'} = \text{NonZero}(v, i, i', j, j', k, k')$ due to Equations $(\ref{exclusive})$, i.e., we are summing 6 variables but using 3 as the bound.

We can formulate $x^{v-}_{ii'jj'kk'} = \text{NonZero}(v, i, i', j, j', k, k') \wedge \text{OddNegOne}(v, i, i', j, j', k, k')$ and $x^{v+}_{ii'jj'kk'} = \text{NonZero}(v, i, i', j, j', k, k') \wedge \text{EvenNegOne}(v, i, i', j, j', k, k')$ by the same technique.

$$
2 x^{v-}_{ii'jj'kk'} \le z^{v}_{ii'jj'kk'} + o^{v}_{ii'jj'kk'} \le 1 + x^{v-}_{ii'jj'kk'}, \quad \forall v \in [1, u], \forall i, i', j, j', k, k' \in [1, m]
$$

$$
2 x^{v+}_{ii'jj'kk'} \le z^{v}_{ii'jj'kk'} + (1 - o^{v}_{ii'jj'kk'}) \le 1 + x^{v+}_{ii'jj'kk'}, \quad \forall v \in [1, u], \forall i, i', j, j', k, k' \in [1, m]
$$

### Complete Model

| Variable              | Description                               | Remark |
| --------------------- | ----------------------------------------- | ------ |
| $r^{v+}_{ij}$         | $\text{bool}(r^{v}_{ij} = 1)$             |        |
| $r^{v-}_{ij}$         | $\text{bool}(r^{v}_{ij} = -1)$            |        |
| $p^{v+}_{ij}$         | $\text{bool}(p^{v}_{ij} = 1)$             |        |
| $p^{v-}_{ij}$         | $\text{bool}(p^{v}_{ij} = -1)$            |        |
| $q^{v+}_{ij}$         | $\text{bool}(q^{v}_{ij} = 1)$             |        |
| $q^{v-}_{ij}$         | $\text{bool}(q^{v}_{ij} = -1)$            |        |
|                       | define alias $\pi^{v}_{ii'jj'kk'} = r^{v}_{ij} p^{v}_{i'k} q^{v}_{k'j'}$ to be used later |  |
| $o^{v}_{ii'jj'kk'}$   | $\left( (o = 1) \Leftrightarrow (\pi \ne 1) \right) \wedge \left( (o = 0) \Leftrightarrow (\pi \ne -1) \right)$ | $o^{v}_{ii'jj'kk'} = \text{OddNegOne}(v, i, i', j, j', k, k')$ |
| $y^{v}_{ii'jj'kk'}$   | auxiliary variable                        |        |
| $z^{v}_{ii'jj'kk'}$   | $\text{bool}(\pi \ne 0)$  | $z^{v}_{ii'jj'kk'} = \text{NonZero}(v, i, i', j, j', k, k')$ |
| $x^{v+}_{ii'jj'kk'}$   | $\text{bool}(\pi = 1)$ | $x^{v+}_{ii'jj'kk'} = z^{v}_{ii'jj'kk'} \wedge e^{v}_{ii'jj'kk'}$ |
| $x^{v-}_{ii'jj'kk'}$   | $\text{bool}(\pi = -1)$   | $x^{v-}_{ii'jj'kk'} = z^{v}_{ii'jj'kk'} \wedge \neg e^{v}_{ii'jj'kk'}$ |

$$
r^{v+}_{ij}, r^{v-}_{ij}, p^{v+}_{ij}, p^{v-}_{ij}, q^{v+}_{ij}, q^{v-}_{ij} \in \{0, 1\}, \quad \forall v \in [1, u], \forall i, j \in [1, m]
$$

$$
e^{v}_{ii'jj'kk'}, y^{v}_{ii'jj'kk'}, z^{v}_{ii'jj'kk'}, x^{v+}_{ii'jj'kk'}, x^{v-}_{ii'jj'kk'} \in \{0, 1\}, \forall v \in [1, u], \forall i, i', j, j', k, k' \in [1, m]
$$

$$
\begin{align}
r^{v+}_{ij} + r^{v-}_{ij} \le 1, \quad \forall v \in [1, u], \forall i, j \in [1, m]\\
p^{v+}_{ij} + p^{v-}_{ij} \le 1, \quad \forall v \in [1, u], \forall i, j \in [1, m]\\
q^{v+}_{ij} + q^{v-}_{ij} \le 1, \quad \forall v \in [1, u], \forall i, j \in [1, m]
\end{align}
$$

$$
r^{v-}_{ij} + p^{v-}_{i'k} + q^{v-}_{k'j'} = 2 y^{v}_{ii'jj'kk'} + o^{v}_{ii'jj'kk'}, \quad \forall v \in [1, u], \forall i, i', j, j', k, k' \in [1, m]
$$

$$
3 z^{v}_{ii'jj'kk'} \le r^{v+}_{ij} + r^{v-}_{ij} + p^{v+}_{i'k} + p^{v-}_{i'k} + q^{v+}_{k'j'} + q^{v-}_{k'j'} \le 2 + z^{v}_{ii'jj'kk'}, \quad \forall v \in [1, u], \forall i, i', j, j', k, k' \in [1, m]
$$

$$
2 x^{v-}_{ii'jj'kk'} \le z^{v}_{ii'jj'kk'} + o^{v}_{ii'jj'kk'} \le 1 + x^{v-}_{ii'jj'kk'}, \quad \forall v \in [1, u], \forall i, i', j, j', k, k' \in [1, m]
$$

$$
2 x^{v+}_{ii'jj'kk'} \le z^{v}_{ii'jj'kk'} + (1 - o^{v}_{ii'jj'kk'}) \le 1 + x^{v+}_{ii'jj'kk'}, \quad \forall v \in [1, u], \forall i, i', j, j', k, k' \in [1, m]
$$

$$
\sum^{u}_{v=1} x^{v+}_{iijjkk} - \sum^{u}_{v=1} x^{v-}_{iijjkk} = 1, \quad \forall i, j, k \in [1, m]
$$

$$
\sum^{u}_{v=1} x^{v+}_{ii'jj'kk'} - \sum^{u}_{v=1} x^{v-}_{ii'jj'kk'} = 0, \quad \forall i, i', j, j', k, k' \in [1, m], (i \ne i') \vee (j \ne j') \vee (k \ne k')
$$


## CNF Encoding

### Encoding Exclusive Or

In order to utilize the state-of-the-art SAT solvers, we need to encode this problem in CNF, where the XOR operators are forbidden.

$$
\begin{align}
r \oplus p \oplus q & \iff (r \wedge p \wedge q) \vee (r \wedge \neg p \wedge \neg q) \vee (\neg r \wedge p \wedge \neg q) \vee (\neg r \wedge \neg p \wedge q)\\
                    & \iff (r \vee p \vee q) \wedge (r \vee \neg p \vee \neg q) \wedge (\neg r \vee p \vee \neg q) \wedge (\neg r \vee \neg p \vee q)
\label{xor2cnf}
\end{align}
$$

Then, we introduce an auxiliary variable $o$ for each XOR expression $r \oplus p \oplus q$ so that we can refer to its result with $o$ instead of applying Equation $(\ref{xor2cnf})$ everywhere.

$$
\begin{align}
(a \rightarrow b)     & \iff (\neg a \vee b)\\
(a \leftrightarrow b) & \iff (\neg a \vee b) \wedge (a \vee \neg b)\\
(a \leftrightarrow b) & \iff (a \odot b) \iff (a \wedge b) \vee (\neg a \wedge \neg b)
\end{align}
$$

$$
\begin{align}
o = r \oplus p \oplus q & \iff (\neg o \vee (r \oplus p \oplus q)) \wedge (o \vee \neg (r \oplus p \oplus q))\\
                        & \iff (o \wedge (r \oplus p \oplus q)) \vee (\neg o \wedge \neg (r \oplus p \oplus q))
\end{align}
$$

### Encoding Counter and Comparer Circuits

...

### Complete CNF Expression

...


## To-do List

- [ ] Encoder.
- [ ] Checker.
  - [ ] Correctness.
  - [ ] Equivalence or isomorphism.


## Future Works

- Try greater $u$.
- Try to minimize the number of addition operations.
- Try to use relax-and-fix method.
  - First determine each term is involved or not, then decide their coefficients.
- Try wider domains for the parameters.
  - Especially power of two, e.g., $..., \pm 4, \pm 2, \pm 0.5, \pm 0.25, ...$
- Try to let the calculation of the intermediates can utilize other intermediates.
  - There must not be cyclic references.
- Try to break the symmetry among different solutions.
  - By swapping the occurrences and the definitions of a pair of intermediate matrices $M_{v}$ and $M_{v'}$, a homogenous solution is found.
    - For each pair of $v, v' \in [1, u]$, do the value swap as $r^{v}_{ij} \leftrightarrow r^{v'}_{ij}, p^{v}_{ij} \leftrightarrow p^{v'}_{ij}, q^{v}_{ij} \leftrightarrow q^{v'}_{ij}, \forall i, j, k \in [1, m]$.
- Try to use the symmetry within single solution.
  - There is a corresponding index pattern $(\boldsymbol{a}_{ij} + ... +\boldsymbol{a}_{i'j'})$ if there is a index pattern $(\boldsymbol{b}_{ij} + ... + \boldsymbol{b}_{i'j'})$ in Strassen's construction.
    - This assumption does not hold in 3x3 case.
- Try column generation.
  - Let $d$ be the size of the domain, e.g., $d = 3$ if $p^{v}_{ij}, q^{v}_{ij}, r^{v}_{ij} \in \{-1, 0, 1\}, \forall v \in [1, u], \forall i, j \in [1, m]$.
  - Naive complexity.
    - The combination of $\boldsymbol{p}$ produces $d^{m^{2}} - 1$ columns.
    - The combination of $\boldsymbol{q}$ produces $d^{m^{2}} - 1$ columns.
    - The combination of $\boldsymbol{r}$ produces $d^{u} - 1$ columns.
  - Empirical complexity.
    - 3x3 case.
      - Assume each sum in each intermediate matrix consists of up to 8 terms.
        - $\sum^{8}_{k=1} ((d - 1)^{k} C^{k}_{m^{2}})$ columns for $\boldsymbol{p}$ and $\boldsymbol{q}$, respectively.
      - Assume each resulting sub-matrix contains up to 8 intermediate matrices.
        - $\sum^{8}_{k=1} ((d - 1)^{k} C^{k}_{u})$ columns for $\boldsymbol{r}$.
